Termination for Hyb without diamond - main lemma done

Normalization/Hyb_NoDiamond.v
@@ -2,63 +2,11 @@ Add LoadPath "..".
 Add LoadPath "../Hybrid".
 Require Import Shared.
 Require Import Hybrid.
+Require Import ListLib.
 
 Open Scope is5_scope.
 Open Scope hybrid_is5_scope.
 Open Scope permut_scope.
-
-Definition normal_form (M: te_Hyb) := value_Hyb M.
-
-Inductive neutral_Hyb: te_Hyb -> Prop :=
-| nHyp: forall n, neutral_Hyb (hyp_Hyb n)
-| nAppl: forall M N, neutral_Hyb (appl_Hyb M N)
-| nUnbox: forall M w, neutral_Hyb (unbox_fetch_Hyb w M)
-| nHere: forall M w, neutral_Hyb M -> neutral_Hyb (get_here_Hyb w M)
-| nULetdia: forall M N w, neutral_Hyb (letdia_get_Hyb w M N)
-.
-
-Lemma value_no_step:
-forall M,
-  value_Hyb M ->
-  forall N w , ~ (M, w) |-> (N, w).
-induction M; intros; intro;
-try inversion H0; inversion H1; subst;
-inversion H; subst; eapply IHM; eauto; try omega.
-Qed.
-
-Lemma neutral_or_value:
-forall M,
-  neutral_Hyb M \/ value_Hyb M.
-induction M; intros;
-try (destruct IHM; [left | right]; constructor; auto).
-left; constructor.
-right; constructor.
-left; constructor.
-right; constructor.
-left; constructor.
-left; constructor.
-Qed.
-
-Inductive SN: te_Hyb -> Prop :=
-| val_SN: forall M, value_Hyb M -> SN M
-| step_SN: forall M w,
-             (forall N, (M , w) |-> (N, w) -> SN N) ->
-             SN M.
-
-
-Fixpoint Red (M: te_Hyb) (A: ty) : Prop :=
-match A with
-| tvar => SN M
-| tarrow A1 A2 =>
-    forall N
-           (H_lc_t: lc_t_Hyb N)
-           (H_lc_w: lc_w_Hyb N)
-           (HRed: Red N A1),
-      Red (appl_Hyb M N) A2
-| tbox A1 => forall w',
-               Red (unbox_fetch_Hyb (fwo w') M) A1
-| tdia A1 => False
-end.
 
 Lemma closed_t_succ_Hyb:
 forall M n,
@@ -98,6 +46,62 @@ forall M N w,
   lc_t_Hyb N.
 intros; eapply lc_t_step_Hyb_preserv; eauto.
 Qed.
+
+Lemma closed_t_succ:
+forall M n,
+  lc_t_n_Hyb n M -> lc_t_n_Hyb (S n) M.
+intros; generalize dependent n;
+induction M; intros; inversion H; subst;
+eauto using lc_t_n_Hyb.
+Qed.
+
+Lemma closed_t_addition:
+forall M n m,
+  lc_t_n_Hyb n M -> lc_t_n_Hyb (n + m) M.
+intros; induction m;
+[ replace (n+0) with n by auto |
+  replace (n + S m) with (S (n+m)) by auto] ;
+try apply closed_t_succ;
+assumption.
+Qed.
+
+Definition normal_form (M: te_Hyb) := value_Hyb M.
+
+Inductive neutral_Hyb: te_Hyb -> Prop :=
+| nHyp: forall n, neutral_Hyb (hyp_Hyb n)
+| nAppl: forall M N, neutral_Hyb (appl_Hyb M N)
+| nUnbox: forall M w, neutral_Hyb (unbox_fetch_Hyb w M)
+| nHere: forall M w, neutral_Hyb M -> neutral_Hyb (get_here_Hyb w M)
+| nULetdia: forall M N w, neutral_Hyb (letdia_get_Hyb w M N)
+.
+
+Lemma value_no_step:
+forall M,
+  value_Hyb M ->
+  forall N w , ~ (M, w) |-> (N, w).
+induction M; intros; intro;
+try inversion H0; inversion H1; subst;
+inversion H; subst; eapply IHM; eauto; try omega.
+Qed.
+
+Lemma neutral_or_value:
+forall M,
+  neutral_Hyb M \/ value_Hyb M.
+induction M; intros;
+try (destruct IHM; [left | right]; constructor; auto).
+left; constructor.
+right; constructor.
+left; constructor.
+right; constructor.
+left; constructor.
+left; constructor.
+Qed.
+
+Inductive SN: te_Hyb -> Prop :=
+| val_SN: forall M, value_Hyb M -> SN M
+| step_SN: forall M w,
+             (forall N, (M , w) |-> (N, w) -> SN N) ->
+             SN M.
 
 Lemma SN_appl:
 forall M N,
@@ -145,6 +149,20 @@ constructor; apply lc_t_step_Hyb in H4; auto.
 omega.
 Qed.
 
+Fixpoint Red (M: te_Hyb) (A: ty): Prop :=
+match A with
+| tvar => SN M
+| tarrow A1 A2 =>
+    forall N
+           (H_lc_t: lc_t_Hyb N)
+           (H_lc_w: lc_w_Hyb N)
+           (HRed: Red N A1),
+      Red (appl_Hyb M N) A2
+| tbox A1 => forall w',
+               Red (unbox_fetch_Hyb (fwo w') M) A1
+| tdia A1 => False
+end.
+
 (* CR 2 *)
 Theorem property_2:
 forall A M M'
@@ -182,7 +200,7 @@ induction A; intros; simpl in *.
 intros; apply step_SN with (w:=fwo x); auto; intros;
 apply H1 with x; auto.
 (* arrow type *)
-intros; apply IHA2; try constructor; auto; intros; simpl in *.
+intros; apply IHA2; try constructor; auto; intros; simpl in *;
 inversion H2; subst; inversion H0; subst; eapply H1; eauto.
 (* box type *)
 intros; apply IHA; try constructor; auto; intros;
@@ -190,7 +208,6 @@ inversion H2; subst; [inversion H0 | ];
 apply H1 with w'; auto.
 
 skip.
-
 Qed.
 
 (* CR 1 *)
@@ -237,7 +254,7 @@ forall A N B
     lc_t_Hyb M ->
     lc_w_Hyb M ->
     Red M A ->
-    Red ([M// bte 0] N) B),
+    Red ([M// bte 0] N) B) ,
   Red (lam_Hyb A N) (A ---> B).
 simpl; intros;
 apply property_3;
@@ -248,21 +265,18 @@ apply HT; auto.
 inversion HT0.
 Qed.
 
-(*
 Lemma reducible_box:
 forall A M
   (lc_M: lc_t_Hyb M)
-  (HT: Red M A),
+  (HT: forall w, Red (M ^w^ (fwo w)) A),
   Red (box_Hyb M) ([*]A).
 simpl; intros;
 apply property_3;
 repeat constructor; auto.
 intros; inversion H; subst.
 apply HT; auto.
-
-inversion H2.
+inversion HT0.
 Qed.
-*)
 
 Fixpoint find_var (L: list (var * ty * te_Hyb)) (x:var) :
                      option (var * ty * te_Hyb) :=
@@ -272,7 +286,14 @@ match L with
   if (eq_var_dec x v) then Some (v, A, M) else find_var L' x
 end.
 
-Fixpoint SL (L: list (var * ty * te_Hyb)) M :=
+Fixpoint find_world (L: list (var * var)) (w:vwo) : option (var * var) :=
+match L with
+| nil => None
+| (w0, w1) :: L' =>
+  if (eq_vwo_dec w (fwo w1)) then Some (w0, w1) else find_world L' w
+end.
+
+Fixpoint SL (L: list (var * ty * te_Hyb)) (W: list (var * var)) M :=
 match M with
 | hyp_Hyb (bte v) => M
 | hyp_Hyb (fte v) =>
@@ -281,71 +302,29 @@ match M with
     | Some (v, A, M) => M
     | None => hyp_Hyb (fte v)
   end
-| lam_Hyb A M => lam_Hyb A (SL L M)
-| appl_Hyb M N => appl_Hyb (SL L M) (SL L N)
-| box_Hyb M => box_Hyb (SL L M)
-| unbox_fetch_Hyb w M => unbox_fetch_Hyb w (SL L M)
-| get_here_Hyb w M => get_here_Hyb w (SL L M)
-| letdia_get_Hyb w M N => letdia_get_Hyb w (SL L M) (SL L N)
-end.
-
-Fixpoint find_world (L: list (var * var)) (w:vwo) : vwo:=
-match L with
-| nil => w
-| (w0, w1) :: L' =>
-  if (eq_vwo_dec w (fwo w0)) then (fwo w1) else find_world L' w
-end.
-
-Fixpoint RL (L: list (var * var)) M :=
-match M with
-| hyp_Hyb v => M
-| lam_Hyb A M => lam_Hyb A (RL L M)
-| appl_Hyb M N => appl_Hyb (RL L M) (RL L N)
-| box_Hyb M => box_Hyb (RL L M)
+| lam_Hyb A M => lam_Hyb A (SL L W M)
+| appl_Hyb M N => appl_Hyb (SL L W M) (SL L W N)
+| box_Hyb M => box_Hyb (SL L W M)
 | unbox_fetch_Hyb w M =>
-  let w' := find_world L w in
-  unbox_fetch_Hyb w' (RL L M)
+  let x := find_world W w in
+  match x with
+      | Some (x0, x1) => unbox_fetch_Hyb (fwo x0) (SL L W M)
+      | None => unbox_fetch_Hyb w (SL L W M)
+  end
 | get_here_Hyb w M =>
-  let w' := find_world L w in
-  get_here_Hyb w' (RL L M)
+  let x := find_world W w in
+  match x with
+      | Some (x0, x1) => get_here_Hyb (fwo x0) (SL L W M)
+      | None => get_here_Hyb w (SL L W M)
+  end
 | letdia_get_Hyb w M N =>
-    let w' := find_world L w in
-    letdia_get_Hyb w' (RL L M) (RL L N)
+  let x := find_world W w in
+  match x with
+      | Some (x0, x1) => letdia_get_Hyb (fwo x0) (SL L W M) (SL L W N)
+      | None => letdia_get_Hyb w (SL L W M) (SL L W N)
+  end
 end.
 
-Lemma Mem_concat_mem_elem:
-forall (G: bg_Hyb) (e:var*ty),
-  Mem e (concat (map snd_ G)) ->
-  exists l, Mem l (map snd_ G) /\ Mem e l.
-induction G; intros; rew_map in *; rew_concat in *.
-rewrite Mem_nil_eq in H; contradiction.
-rewrite Mem_app_or_eq in H; destruct H.
-exists (snd a); split; auto; apply Mem_here.
-destruct (IHG e); auto; destruct H0; exists x; split; auto.
-rewrite Mem_cons_eq; right; auto.
-Qed.
-(*
-Lemma ok_Hyb_Mem_Mem_eq':
-  forall (G : bg_Hyb)(v : var) (A B : ty),
-    ok_Hyb G  ->
-    Mem (v, A) (concatG -> Mem (v,B) G ->
-    A = B.
-induction G; intros.
-rewrite Mem_nil_eq in H0; contradiction.
-rewrite Mem_cons_eq in *; destruct H0; destruct H1; subst.
-inversion H1; subst; auto.
-inversion H; subst; apply Mem_split in H1; destruct H1 as (hd, (tl, H1));
-assert (hd & (v, B) ++ tl *=* (v, B) :: hd ++ tl) by permut_simpl;
-rewrite H1 in H6; apply ok_Hyb_permut with (G':= (v, B) :: hd ++ tl) in H6;
-auto; inversion H6; subst; elim H8; apply Mem_here.
-inversion H; subst; apply Mem_split in H0; destruct H0 as (hd, (tl, H0));
-assert (hd & (v, A) ++ tl *=* (v, A) :: hd ++ tl) by permut_simpl;
-rewrite H0 in H6; apply ok_Hyb_permut with (G':= (v, A) :: hd ++ tl) in H6;
-auto; inversion H6; subst; elim H8; apply Mem_here.
-eapply IHG; eauto.
-inversion H; subst; eapply ok_Hyb_used_weakening; eauto.
-Qed.
-*)
 Fixpoint OkL (L: list (var * ty * te_Hyb)) U :=
 match L with
 | nil => True
@@ -365,11 +344,11 @@ forall L U w,
 Admitted.
 
 Lemma Mem_Red_Hyp:
-forall L v A M,
+forall L v A M W,
   (forall (a : var) (b : ty) (c : te_Hyb), Mem (a, b, c) L → Red c b) ->
   Mem (v, A, M) L ->
   OkL L nil ->
-  SL L (hyp_Hyb (fte v)) = M.
+  SL L W (hyp_Hyb (fte v)) = M.
 induction L; intros; rew_map in *.
 rewrite Mem_nil_eq in H0; contradiction.
 destruct a; destruct p; simpl in *; case_if.
@@ -379,7 +358,7 @@ destruct H1.
 apply OkL_used_notin with (U:=v0::nil) in H0;
   [contradiction | auto | apply Mem_here ].
 destruct H1.
-apply IHL with A.
+apply IHL with A; auto.
 intros; apply H with a; rewrite Mem_cons_eq; right; auto.
 rewrite Mem_cons_eq in H0; destruct H0; auto; inversion H0; subst;
 elim H2; auto.
@@ -387,12 +366,12 @@ apply OkL_weaken in H3; auto.
 Qed.
 
 Lemma SL_hyp:
-  forall L G Gamma w v A,
+  forall L G Gamma w v A W,
   OkL L nil ->
   concat (Gamma::(map snd_ G)) *=* map fst_ L ->
   (forall a b c, Mem (a, b, c) L -> Red c b) ->
   G |= (w, Gamma) |- hyp_Hyb (fte v) ::: A ->
-  Red (SL L (hyp_Hyb (fte v))) A.
+  Red (SL L W (hyp_Hyb (fte v))) A.
 intros.
 assert (Mem (v, A) (map fst_ L)).
   apply Mem_permut with (l:= concat (Gamma::map snd_ G)); auto;
@@ -408,31 +387,13 @@ assert (exists M, Mem (v, A, M) L).
   exists x; rewrite Mem_cons_eq; right; auto.
 destruct H4.
 assert (Mem (v, A ,x) L) by auto;
-apply Mem_Red_Hyp in H4; auto;
+apply Mem_Red_Hyp with (W:=W) in H4; auto;
 rewrite H4; apply H1 with v; auto.
-Qed.
-
-Lemma closed_t_succ:
-forall M n,
-  lc_t_n_Hyb n M -> lc_t_n_Hyb (S n) M.
-intros; generalize dependent n;
-induction M; intros; inversion H; subst;
-eauto using lc_t_n_Hyb.
-Qed.
-
-Lemma closed_t_addition:
-forall M n m,
-  lc_t_n_Hyb n M -> lc_t_n_Hyb (n + m) M.
-intros; induction m;
-[ replace (n+0) with n by auto |
-  replace (n + S m) with (S (n+m)) by auto] ;
-try apply closed_t_succ;
-assumption.
 Qed.
 
 Lemma SL_nil:
 forall M,
-  SL nil M = M.
+  SL nil nil M = M.
 induction M; intros; simpl in *;
 try erewrite IHM || (erewrite IHM1; try erewrite IHM2); eauto.
 destruct v; auto.
@@ -472,10 +433,10 @@ rewrite Mem_cons_eq; right; apply IHL; auto.
 Qed.
 
 Lemma lc_SL:
-forall M L n,
+forall M L W n,
   lc_t_n_Hyb n M ->
   (forall a b c, Mem (a,b,c) L -> lc_t_Hyb c) ->
-  lc_t_n_Hyb n (SL L M).
+  lc_t_n_Hyb n (SL L W M).
 induction M; intros; simpl in *;
 try (inversion H; subst; constructor; eapply IHM; eauto).
 destruct v; inversion H; subst.
@@ -486,14 +447,19 @@ rewrite H1. replace n with (0+n) by omega.
 apply closed_t_addition; apply H0 with v x. apply find_var_Mem; auto.
 rewrite NotMem_find_var; auto.
 inversion H; subst; constructor; [apply IHM1 | apply IHM2]; auto.
-inversion H; subst; constructor; [apply IHM2 | apply IHM1]; auto.
+destruct (find_world W v); simpl in *; try destruct p; constructor; auto;
+apply IHM; inversion H; eauto.
+destruct (find_world W v); simpl in *; try destruct p; constructor; auto;
+apply IHM; inversion H; eauto.
+destruct (find_world W v); simpl in *; try destruct p; constructor; auto;
+inversion H; subst; [apply IHM2 | apply IHM1 | apply IHM2 | apply IHM1 ]; auto.
 Qed.
 
 Lemma lc_w_SL:
-forall M L n,
+forall M L W n,
   lc_w_n_Hyb n M ->
   (forall a b c, Mem (a,b,c) L -> lc_w_Hyb c) ->
-  lc_w_n_Hyb n (SL L M).
+  lc_w_n_Hyb n (SL L W M).
 induction M; intros; simpl in *;
 try (inversion H; subst; constructor; eapply IHM; eauto).
 destruct v; inversion H; subst.
@@ -504,17 +470,20 @@ rewrite H1. replace n with (0+n) by omega.
 apply closed_w_addition; apply H0 with v x. apply find_var_Mem; auto.
 rewrite NotMem_find_var; auto.
 inversion H; subst; constructor; [apply IHM1 | apply IHM2]; auto.
-inversion H; subst; constructor; try omega; auto; apply IHM; auto.
-inversion H; subst; constructor; try omega; auto; apply IHM; auto.
-inversion H; subst; constructor; try omega; auto.
+destruct (find_world W v); simpl in *; try destruct p;
+inversion H; constructor; auto; apply IHM; auto.
+destruct (find_world W v); simpl in *; try destruct p;
+inversion H; constructor; auto; apply IHM; auto.
+destruct (find_world W v); simpl in *; try destruct p;
+inversion H; constructor; auto; apply IHM; auto.
 Qed.
 
 Lemma SL_bte_subst:
-forall L0 M x k,
+forall L0 W M x k,
   ~ Mem x (map fst_ (map fst_ L0)) ->
   (forall v a m, Mem (v, a, m) L0 -> lc_t_Hyb m) ->
-  [hyp_Hyb (fte x) // bte k](SL L0 M) =
-  SL L0 [hyp_Hyb (fte x) // bte k]M.
+  [hyp_Hyb (fte x) // bte k](SL L0 W M) =
+  SL L0 W [hyp_Hyb (fte x) // bte k]M.
 induction M; intros; simpl in *;
 try rewrite IHM || (rewrite IHM1; try rewrite IHM2); auto.
 case_if; simpl.
@@ -526,12 +495,24 @@ simpl; repeat case_if; auto.
 apply Mem_find_var in m; destruct m as (a, (b, m)); rewrite m; simpl.
 rewrite closed_subst_t_Hyb_bound with (n:=0); auto; try omega;
 apply H0 with v a; apply find_var_Mem; auto.
+destruct (find_world W v); simpl in *; try destruct p; simpl;
+try erewrite IHM; eauto.
+destruct (find_world W v); simpl in *; try destruct p; simpl;
+try erewrite IHM; eauto.
+destruct (find_world W v); simpl in *; try destruct p; simpl;
+try erewrite IHM1; try erewrite IHM2; eauto.
 Qed.
 
 Fixpoint FV_L (L: list (var * ty * te_Hyb)) :=
 match L with
 | nil => \{}
 | (v, A, M) :: L' => free_vars_Hyb M \u FV_L L'
+end.
+
+Fixpoint FW_L (L: list (var * ty * te_Hyb)) :=
+match L with
+| nil => \{}
+| (v, A, M) :: L' => free_worlds_Hyb M \u FW_L L'
 end.
 
 Lemma notin_FV_notin_elem:
@@ -546,12 +527,57 @@ destruct a; destruct p; rewrite notin_union in H; destruct H;
 apply IHL with (a:=a0) (b:=b); auto.
 Qed.
 
-Lemma SL_extend:
-forall M L0 x A N,
+Lemma notin_FW_notin_elem:
+forall x L,
+  x \notin FW_L L ->
+  forall a b c, Mem (a,b,c) L -> x \notin free_worlds_Hyb c.
+induction L; intros; simpl in *.
+rewrite Mem_nil_eq in *; contradiction.
+rewrite Mem_cons_eq in H0; destruct H0; [inversion H0; subst | ].
+rewrite notin_union in H; destruct H; auto.
+destruct a; destruct p; rewrite notin_union in H; destruct H;
+apply IHL with (a:=a0) (b:=b); auto.
+Qed.
+
+Lemma Mem_find_world:
+  forall W w,
+    Mem w (map snd_ W) ->
+    exists w', find_world W (fwo w) = Some (w', w).
+induction W; intros; [ rewrite Mem_nil_eq in *; contradiction | ];
+destruct a; rew_map in *; simpl in *.
+subst; rewrite Mem_cons_eq in H.
+destruct H; subst.
+exists v; case_if; auto.
+case_if; [inversion H0; subst | ].
+exists v; auto.
+apply IHW; auto.
+Qed.
+
+Lemma NotMem_find_world:
+  forall W w,
+    ~Mem w (map snd_ W) ->
+    find_world W (fwo w) = None.
+induction W; intros; simpl in *; auto;
+destruct a; rew_map in *; simpl in *; case_if.
+inversion H0; subst; elim H; apply Mem_here.
+apply IHW; intro; elim H; rewrite Mem_cons_eq; right; auto.
+Qed.
+
+Lemma find_world_Mem:
+forall W w w',
+  find_world W (fwo w) = Some (w', w) -> Mem (w', w) W.
+induction W; intros; [inversion H; subst | ].
+destruct a; simpl in *; case_if.
+inversion H; subst; apply Mem_here.
+rewrite Mem_cons_eq; right; apply IHW; auto.
+Qed.
+
+Lemma SL_extend_L:
+forall M L0 W x A N,
   x \notin FV_L L0 ->
   ~Mem x (map fst_ (map fst_ L0)) ->
-  SL ((x, A, N) :: L0) M =
-  [N // fte x](SL L0 M).
+  SL ((x, A, N) :: L0) W M =
+  [N // fte x](SL L0 W M).
 induction M; intros; simpl in *;
 try rewrite IHM || (rewrite IHM1; try rewrite IHM2); auto.
 destruct v; simpl; repeat case_if; auto.
@@ -563,6 +589,60 @@ apply Mem_find_var in m; destruct m as (a, (b, m)); rewrite m; simpl.
 rewrite closed_subst_t_Hyb_free; auto.
 apply notin_FV_notin_elem with L0 v a; eauto.
 apply find_var_Mem; eauto.
+destruct (find_world W v); simpl; try destruct p; auto.
+destruct (find_world W v); simpl; try destruct p; auto.
+destruct (find_world W v); simpl; try destruct p; auto.
+Qed.
+
+Lemma find_world_bound_None:
+forall W k,
+  find_world W (bwo k) = None.
+induction W; intros; simpl; auto; destruct a; case_if; auto.
+Qed.
+
+Lemma Mem_fst_:
+forall A B (a:A) (b:B) L,
+Mem (a, b) L -> Mem a (map fst_ L).
+induction L; intros; [rewrite Mem_nil_eq in *; contradiction| ];
+rew_map in *; simpl in *; rewrite Mem_cons_eq in *; destruct H; subst;
+[left | right]; auto.
+Qed.
+
+Lemma SL_extend_W:
+forall M L W w0 w1,
+  ~ Mem w1 (map snd_ W) ->
+  w1 \notin FW_L L ->
+  ~ Mem w1 (map fst_ W) ->
+  SL L ((w0, w1)::W) M =
+  {{fwo w0 // fwo w1}}(SL L W M).
+induction M; intros; simpl in *; repeat (case_if; simpl in *);
+try rewrite IHM || (rewrite IHM1; try rewrite IHM2); auto;
+try (apply NotMem_find_world in H; rewrite H; simpl; case_if; auto).
+destruct v; simpl; repeat case_if; auto;
+destruct (Mem_dec var (map fst_ (map fst_ L)) v);
+try apply eq_var_dec; [ | rewrite NotMem_find_var]; auto;
+simpl; repeat case_if; auto;
+apply Mem_find_var in m; destruct m as (a, (b, m)); rewrite m; simpl;
+rewrite closed_subst_w_Hyb_free; auto;
+apply notin_FW_notin_elem with L v a; eauto; apply find_var_Mem; eauto.
+destruct v; [rewrite find_world_bound_None | ]; simpl; repeat case_if; auto;
+destruct (Mem_dec var (map snd_ W) v); [ apply eq_var_dec | | ];
+[ | rewrite NotMem_find_world]; auto; simpl; repeat case_if; auto;
+apply Mem_find_world in m; destruct m as (wa, m); rewrite m; simpl;
+case_if; auto; inversion H3; subst;
+apply find_world_Mem in m; apply Mem_fst_ in m; contradiction.
+destruct v; [rewrite find_world_bound_None | ]; simpl; repeat case_if; auto;
+destruct (Mem_dec var (map snd_ W) v); [ apply eq_var_dec | | ];
+[ | rewrite NotMem_find_world]; auto; simpl; repeat case_if; auto;
+apply Mem_find_world in m; destruct m as (wa, m); rewrite m; simpl;
+case_if; auto; inversion H3; subst;
+apply find_world_Mem in m; apply Mem_fst_ in m; contradiction.
+destruct v; [rewrite find_world_bound_None | ]; simpl; repeat case_if; auto;
+destruct (Mem_dec var (map snd_ W) v); [ apply eq_var_dec | | ];
+[ | rewrite NotMem_find_world]; auto; simpl; repeat case_if; auto;
+apply Mem_find_world in m; destruct m as (wa, m); rewrite m; simpl;
+case_if; auto; inversion H3; subst;
+apply find_world_Mem in m; apply Mem_fst_ in m; contradiction.
 Qed.
 
 Lemma OkL_fresh:
@@ -572,25 +652,11 @@ forall L x a V,
   OkL ((x, a, V):: L) nil.
 Admitted.
 
-Lemma value_Hyb_rename:
-forall M w0 w1,
-  value_Hyb M -> value_Hyb {{fwo w0//fwo w1}}M.
-intros; induction H; simpl in *; constructor; auto.
-Qed.
-
-Lemma SN_rename_w:
-forall N w0 w1,
-SN N -> SN {{fwo w0//fwo w1}}N.
-intros; induction H.
-constructor; apply value_Hyb_rename; auto.
-apply step_SN with w; intros.
-Admitted.
-
 Lemma SL_subst_w:
-forall M L w k,
+forall M L W w k,
   (forall a b c, Mem (a, b, c) L -> lc_w_Hyb c) ->
-  {{w // bwo k}}(SL L M) =
-  SL L {{w//bwo k}}M.
+  {{w // bwo k}}(SL L W M) =
+  SL L W {{w//bwo k}}M.
 induction M; intros; simpl; auto;
 try (erewrite IHM || (erewrite IHM1; try erewrite IHM2));
 eauto.
@@ -602,7 +668,36 @@ rewrite H0; apply find_var_Mem in H0;
 rewrite closed_subst_w_Hyb_bound with (n:=0); auto;
 try omega; apply H with v x; auto.
 apply NotMem_find_var in n; rewrite n; simpl; auto.
+repeat case_if.
+Admitted.
+
+(*
+Lemma rename_world_subst_t:
+forall M w0 w1 N v,
+  {{fwo w0 // fwo w1}} ([N // v] M) =
+  [{{fwo w0//fwo w1}}N//v] {{fwo w0//fwo w1}}M.
+induction M; intros; simpl in *; repeat case_if; auto;
+try erewrite IHM || (erewrite IHM1; try erewrite IHM2); eauto.
 Qed.
+
+Lemma rename_reorder:
+forall M w0 w1 k,
+{{fwo w1 // fwo w0}}({{fwo w0 // bwo k}}M)  =
+{{fwo w1 // bwo k}} ({{fwo w1 // fwo w0}} M).
+induction M; intros; simpl in *; repeat case_if; auto;
+try erewrite IHM || (erewrite IHM1; try erewrite IHM2); eauto.
+Qed.
+
+Lemma reorder':
+forall M ctx'' w0 k w1,
+  ctx'' <> fwo w0 ->
+  {{ctx'' // bwo k}}({{fwo w1 // fwo w0}}M) =
+  {{fwo w1 // fwo w0}}({{ctx'' // bwo k}}M).
+induction M; intros; simpl in *; repeat case_if; auto;
+try erewrite IHM || (erewrite IHM1; try erewrite IHM2); eauto;
+destruct ctx''; simpl in *; auto; discriminate.
+Qed.
+*)
 
 Theorem main_theorem:
 forall G Gamma M A w,
@@ -615,23 +710,22 @@ forall G Gamma M A w,
     (forall a b c, Mem (a,b,c) L -> lc_t_Hyb c) ->
     (forall a b c, Mem (a,b,c) L -> lc_w_Hyb c) ->
     (forall a b c, Mem (a,b,c) L -> Red c b) ->
-    Red (SL L (RL W M)) A.
+    Red (SL L W M) A.
 intros G Gamma M A w LC_t LC_w HT.
 remember (w, Gamma) as Ctx; generalize dependent w;
 generalize dependent Gamma.
 induction HT; intros; inversion HeqCtx; subst.
 (* hyp *)
-replace (RL W (hyp_Hyb (fte v))) with (hyp_Hyb (fte v)) by (simpl; auto).
 inversion LC_t; subst; try omega;
 apply SL_hyp with G Gamma0 w0; auto;
 constructor; auto.
 (* lam *)
 unfold open_t_Hyb in *;
-assert (exists x, x \notin L \u free_vars_Hyb (SL L0 M) \u
+assert (exists x, x \notin L \u free_vars_Hyb (SL L0 W M) \u
        from_list (map fst_ (map fst_ L0)) \u FV_L L0) by apply Fresh;
 destruct H5.
 assert (forall V, Red V A -> lc_t_Hyb V -> lc_w_Hyb V ->
-           Red (SL ((x, A, V) :: L0) (RL W [hyp_Hyb (fte x) // bte 0]M)) B).
+           Red (SL ((x, A, V) :: L0) W [hyp_Hyb (fte x) // bte 0]M) B).
 intros; apply H with ((x,A)::Gamma0) w0; auto.
 apply lc_t_subst_t_Hyb_bound; [ constructor | inversion LC_t]; auto.
 apply lc_w_subst_t_Hyb; [ constructor | inversion LC_w]; auto.
@@ -648,22 +742,15 @@ inversion H9; subst; auto.
 eapply H4; eauto.
 simpl in *; intros; apply property_3.
 constructor; auto; constructor; apply lc_SL; auto; inversion LC_t; auto.
-Lemma RL_lc_t:
-forall k M W,
-  lc_t_n_Hyb k M ->
-  lc_t_n_Hyb k (RL W M).
-Admitted.
-simpl; apply RL_lc_t; auto.
 constructor.
 intros; inversion H7; subst.
 unfold open_t_Hyb in *.
 rewrite subst_t_Hyb_neutral_free with (v:=x); auto.
-replace ([N // fte x]([hyp_Hyb (fte x) // bte 0](SL L0 (RL W M)))) with
-  (SL ((x, A, N)::L0) (RL W [hyp_Hyb (fte x) // bte 0] M)).
+replace ([N // fte x]([hyp_Hyb (fte x) // bte 0](SL L0 W M))) with
+  (SL ((x, A, N)::L0) W [hyp_Hyb (fte x) // bte 0] M).
 apply H6; auto.
 rewrite SL_bte_subst; auto; [ | apply notin_Mem; auto].
-rewrite SL_extend; auto.
-
+rewrite SL_extend_L; auto.
 apply notin_Mem; auto.
 inversion HT0.
 (* appl *)
@@ -673,30 +760,42 @@ apply lc_SL; auto.
 apply lc_w_SL; auto.
 apply IHHT2 with Gamma0 w0; auto.
 (* box *)
-simpl in *; inversion LC_t; inversion LC_w; subst; intros; apply property_3.
-constructor; constructor; apply lc_SL; auto.
-constructor.
-intros; inversion H5; subst.
-unfold open_w_Hyb in *;
-assert (exists w, w \notin L) by apply Fresh.
-destruct H6.
-specialize H with x Gamma0 w0 w;
-apply H with nil x  L0 in H6; auto.
-Focus 4. rew_concat; rewrite <- H1; rew_map; rew_concat; simpl; auto.
-
-
-rewrite <- subst_w_Hyb_neutral_free with (w0:=x).
+replace (SL L0 W (box_Hyb M)) with (box_Hyb (SL L0 W M)) by (simpl; auto).
+apply reducible_box.
+inversion LC_t; subst; apply lc_SL; auto.
+unfold open_w_Hyb in *.
+assert (exists w, w \notin L \u free_worlds_Hyb (SL L0 W M) \u FW_L L0
+       \u from_list (map fst_ W) \u from_list (map snd_ W))
+  by apply Fresh. destruct H5.
+intros.
+rewrite <- subst_w_Hyb_neutral_free with (w0:=x); eauto;
 rewrite SL_subst_w; auto.
-apply H with Gamma0 x; auto.
-rew_concat in *; rewrite <- H; permut_simpl.
-inversion H6.
+replace ({{fwo w // fwo x}}(SL L0 W {{fwo x // bwo 0}}M))
+        with (SL L0 ((w,x)::W) {{fwo x // bwo 0}}M).
+apply H with nil x; auto.
+inversion LC_t; subst; apply lc_t_subst_w_Hyb; auto.
+inversion LC_w; subst; apply lc_w_subst_Hyb; auto.
+rew_concat; rew_map; rewrite <- H1; rew_map; rew_concat; permut_simpl.
+rewrite SL_extend_W; auto; apply notin_Mem; auto.
 (* unbox *)
-simpl in *;
-inversion LC; subst; apply IHHT; auto.
+simpl in *; inversion LC_t; inversion LC_w; subst;
+destruct (find_world W (fwo w0)); try destruct p;
+apply IHHT with Gamma0 w0; auto.
 (* unbox-fetch *)
-simpl in *;
-inversion LC; subst; apply IHHT; auto;
-rewrite <- H0; apply PPermut_concat_permut; rewrite <- H; PPermut_Hyb_simpl.
+simpl in *; inversion LC_t; inversion LC_w; subst;
+destruct (find_world W (fwo w)); try destruct p;
+apply IHHT with Gamma w; auto.
+rewrite <- H1; rew_map; rew_concat; simpl; permut_simpl;
+repeat rewrite flat_map_concat; simpl;
+transitivity (flat_map snd_ ((w, Gamma)::G)).
+rew_flat_map; auto. apply flat_map_PPermut_Hyb; rewrite <- H.
+PPermut_Hyb_simpl.
+rewrite <- H1; rew_map; rew_concat; simpl; permut_simpl;
+repeat rewrite flat_map_concat; simpl;
+transitivity (flat_map snd_ ((w, Gamma)::G)).
+rew_flat_map; auto. apply flat_map_PPermut_Hyb; rewrite <- H.
+PPermut_Hyb_simpl.
+skip. skip. skip. skip.
 Qed.
 
 Lemma lc_t_n_Hyb_subst_t:
@@ -708,30 +807,25 @@ induction N; intros; simpl in *; try destruct v; constructor;
 repeat case_if; try inversion H1; subst; try omega;
 inversion H0; subst; eauto.
 apply IHN with (M:=M); eauto; apply closed_t_succ_Hyb; auto.
-Qed.
-
-Lemma types_Hyb_lc_t_Hyb:
-forall G Gamma M A,
-  G |= Gamma |- M ::: A -> lc_t_Hyb M.
-intros; induction H; constructor; try apply IHHT;
-unfold open_Hyb in *; auto.
-assert (exists x, x \notin L) by apply Fresh; destruct H1;
-assert (x \notin L) by auto;
-specialize H0 with x; apply H0 in H1;
-apply lc_t_n_Hyb_subst_t in H0; auto; constructor.
+apply IHN2 with (M:=M); eauto; apply closed_t_succ_Hyb; auto.
+apply IHN2 with (M:=M); eauto; apply closed_t_succ_Hyb; auto.
 Qed.
 
 Theorem SN_Lang:
-forall G M A,
-  emptyEquiv_Hyb G |= nil |- M ::: A ->
+forall G M A w,
+  emptyEquiv_Hyb G |= (w, nil) |- M ::: A ->
   SN M.
 intros; apply property_1 with A.
 apply types_Hyb_lc_t_Hyb in H; auto.
-apply main_theorem with (L:=nil) in H.
+apply types_Hyb_lc_w_Hyb in H; auto.
+apply main_theorem with (L:=nil) (W:=nil) in H.
 rewrite SL_nil in H; auto.
 apply types_Hyb_lc_t_Hyb in H; auto.
+apply types_Hyb_lc_w_Hyb in H; auto.
+constructor.
 rew_concat; rew_map; clear H M A.
-induction G; simpl; rew_concat; auto.
+induction G; simpl; rew_concat; auto; destruct a; auto.
+intros; rewrite Mem_nil_eq in *; contradiction.
 intros; rewrite Mem_nil_eq in *; contradiction.
 intros; rewrite Mem_nil_eq in *; contradiction.
 Qed.
